examples/metatheory/pEMFstar.fst
@@ -1,0 +1,346 @@
+module PEMFstar
+
+
+type universe_level = nat
+
+type var = nat
+type universes = list universe_level
+
+type term =
+ | Var : var -> universes -> term
+ | Const : const -> universes -> term
+ | Type_ : universe_level -> term
+ | App : term -> term -> term
+ | Lam : term -> term -> term
+ | Prod : term -> comp -> term
+ | Refine : term -> term -> term
+
+and comp =
+  | Tot_ : term -> comp
+  | Pure_ : term -> term -> comp
+
+and const =
+  (* Natural numbers *)
+  | Nat : const
+  | Zero : const
+  | Succ : const
+  | NatElim : const
+
+  (* Equality *)
+  | Eq : const
+  | Refl : const
+  | EqElim : const
+
+type sub = var -> universes -> Tot term
+type renaming (s:sub) = (forall (x:var) (uvs:universes) . Var? (s x uvs))
+
+let b2i b = if b then 0 else 1
+
+let is_renaming (s:sub)
+  : Ghost nat (requires True) (ensures (fun n -> renaming s ==> n = 0 /\ ~(renaming s) ==> n = 1))
+= b2i (FStar.StrongExcludedMiddle.strong_excluded_middle (renaming s))
+
+let is_evar (e:term) = b2i (Var? e)
+
+let sub_id : s:sub{renaming s} = Var
+let sub_inc : s:sub{renaming s} = fun x uvs -> Var (x+1) uvs
+let sub_dec : s:sub{renaming s} = fun x uvs -> if x = 0 then Var x uvs else Var (x - 1) uvs
+let sub_inc_above (y:var) : s:sub{renaming s} = fun x uvs -> if x < y then Var x uvs else Var (x+1) uvs
+
+let rec subst (s:sub) (e:term)
+  : Pure term
+    (requires True)
+    (ensures (fun e' -> renaming s /\ Var? e ==> Var? e'))
+    (decreases %[is_evar e ; is_renaming s ; 1 ; e])
+=
+  match e with
+  | Var x l -> s x l
+  | Const _ _
+  | Type_ _ -> e
+  | App e1 e2 -> App (subst s e1) (subst s e2)
+  | Lam t e -> Lam (subst s t) (subst (sub_lam s) e)
+  | Prod t1 c -> Prod (subst s t1) (subst_comp (sub_lam s) c)
+  | Refine t1 t2 -> Refine (subst s t1) (subst (sub_lam s) t2)
+
+and sub_lam (s:sub)
+  : Tot (s':sub{renaming s ==> renaming s'})
+    (decreases %[1; is_renaming s ; 0 ; ()])
+=
+  fun y uvs -> if y = 0 then Var y uvs else subst sub_inc (s (y - 1) uvs)
+
+and subst_comp (s:sub) (c:comp)
+  : Tot comp
+  (decreases %[1; is_renaming s ; 1 ; c])
+=
+  match c with
+  | Tot_ t -> Tot_ (subst s t)
+  | Pure_ t wp -> Pure_ (subst s t) (subst s wp)
+
+
+module Ext = FStar.FunctionalExtensionality
+
+(* Substitution extensional; trivial with the extensionality axiom *)
+val subst_extensional: s1:sub -> s2:sub{Ext.feq s1 s2} -> e:term ->
+                        Lemma (requires True) (ensures (subst s1 e = subst s2 e))
+                       (* [SMTPat (subst s1 e);  SMTPat (subst s2 e)] *)
+let subst_extensional s1 s2 e = ()
+
+let sub_lam_hoist (t:term) (e:term) (s:sub)
+  : Lemma (requires True)
+    (ensures (subst s (Lam t e) = Lam (subst s t) (subst (sub_lam s) e)))
+= ()
+
+let sub_prod_hoist (t:term) (c:comp) (s:sub)
+  : Lemma (subst s (Prod t c) = Prod (subst s t) (subst_comp (sub_lam s) c))
+= ()
+
+let sub_refine_hoist (t:term) (phi:term) (s:sub)
+  : Lemma (subst s (Refine t phi) = Refine (subst s t) (subst (sub_lam s) phi))
+= ()
+
+let sub_beta (e:term) : sub = fun y uvs -> if y = 0 then e else Var (y-1) uvs
+let subst_beta (e:term) : term -> term = subst (sub_beta e)
+
+
+(* Identity *)
+
+let sub_lam_id () : Lemma (sub_lam sub_id == sub_id)
+=
+  let aux (y:var) (uvs:universes) : Lemma (sub_lam sub_id y uvs = sub_id y uvs) =
+    if y = 0 then () else ()
+  in
+  Ext.intro_feq2 (sub_lam sub_id) sub_id aux
+
+let rec subst_id (e:term)
+  : Lemma (subst sub_id e = e)
+= match e with
+  | Var _ _ -> ()
+  | Const _ _
+  | Type_ _ -> ()
+  | App e1 e2 -> subst_id e1 ; subst_id e2
+  | Lam t e -> subst_id t ; sub_lam_id () ; subst_id e ; sub_lam_hoist t e sub_id
+  | Prod t c -> subst_id t ; sub_lam_id () ; subst_id_comp c ; sub_prod_hoist t c sub_id
+  | Refine t e -> subst_id t ; sub_lam_id () ; subst_id e ; sub_refine_hoist t e sub_id
+
+and subst_id_comp (c:comp)
+  : Lemma (subst_comp sub_id c = c)
+= match c with
+  | Tot_ t -> subst_id t
+  | Pure_ t wp -> subst_id t ; subst_id wp
+
+let sub_comp (s1 s2 : sub) : sub = fun y uvs -> subst s2 (s1 y uvs)
+
+let sub_comp_id_left (s:sub)
+  : Lemma (sub_comp sub_id s == s)
+= let h (y:var) (uvs:universes) : Lemma (sub_comp sub_id s y uvs == s y uvs) = () in
+  Ext.intro_feq2 (sub_comp sub_id s) s h
+
+let sub_comp_id_right (s:sub)
+  : Lemma (sub_comp s sub_id == s)
+=
+  let h (y:var) (uvs:universes) : Lemma (sub_comp s sub_id y uvs == s y uvs) =
+    subst_id (s y uvs)
+  in
+  Ext.intro_feq2 (sub_comp s sub_id) s h
+
+
+(* unneeded *)
+let sub_inc_sub_dec_id_retract () : Lemma (sub_comp sub_inc sub_dec == sub_id)
+= let h (y:var) (uvs:universes) : Lemma (sub_comp sub_inc sub_dec y uvs == sub_id y uvs) = () in
+  Ext.intro_feq2 (sub_comp sub_inc sub_dec) sub_id h
+
+
+(* Associativity of substitution *)
+
+let sub_comp_inc (s:sub)
+  : Lemma (sub_comp s sub_inc == sub_comp sub_inc (sub_lam s))
+= let s1 = sub_comp s sub_inc in
+  let s2 = sub_comp sub_inc (sub_lam s) in
+  let h (y:var) (uvs:universes) : Lemma (s1 y uvs == s2 y uvs) = () in
+  Ext.intro_feq2 s1 s2 h
+
+let rec subst_sub_comp (s1 s2 : sub) (e:term)
+  : Lemma (requires True)
+    (ensures (subst (sub_comp s1 s2) e = subst s2 (subst s1 e)))
+    (decreases %[is_evar e ; is_renaming s1 ; is_renaming s2 ; 1 ; e])
+= match e with
+  | Var _ _ -> ()
+  | Const _ _
+  | Type_ _ -> ()
+  | App e1 e2 -> subst_sub_comp s1 s2 e1 ; subst_sub_comp s1 s2 e2
+  | Lam t e ->
+    subst_sub_comp s1 s2 t ; sub_lam_comp s1 s2 ; subst_sub_comp (sub_lam s1) (sub_lam s2) e
+  | Prod t c ->
+    subst_sub_comp s1 s2 t ; sub_lam_comp s1 s2 ; subst_comp_sub_comp (sub_lam s1) (sub_lam s2) c
+  | Refine t e ->
+    subst_sub_comp s1 s2 t ; sub_lam_comp s1 s2 ; subst_sub_comp (sub_lam s1) (sub_lam s2) e
+
+and sub_lam_comp (s1 s2 : sub)
+  : Lemma (requires True)
+    (ensures (sub_lam (sub_comp s1 s2) == sub_comp (sub_lam s1) (sub_lam s2)))
+    (decreases %[1 ; is_renaming s1 ; is_renaming s2 ; 0 ; ()])
+=
+  let h (y : var) (uvs:universes)
+    : Lemma (sub_lam (sub_comp s1 s2) y uvs == sub_comp (sub_lam s1) (sub_lam s2) y uvs)
+  = if y = 0 then () else begin
+      (* sub_lam (sub_comp s1 s2) y uvs *)
+      (* = subst sub_inc ((sub_comp s1 s2) (y -1) uvs) *)
+      (* = subst sub_inc (subst s2 (s1 (y - 1) uvs)) *)
+
+      subst_sub_comp s2 sub_inc (s1 (y - 1) uvs) ;
+
+      (* = subst (sub_comp s2 sub_inc) (s1 (y-1) uvs) *)
+
+      sub_comp_inc s2 ;
+      subst_extensional (sub_comp s2 sub_inc) (sub_comp sub_inc (sub_lam s2)) (s1 (y-1) uvs) ;
+
+      (* = subst (sub_comp sub_inc (sub_lam s2)) (s1 (y-1) uvs) *)
+
+      subst_sub_comp sub_inc (sub_lam s2) (s1 (y - 1) uvs)
+
+      (* = subst (sub_lam s2) (subst sub_inc (s1 (y-1) uvs)) *)
+      (* = sub_comp (sub_lam s1) (sub_lam s2) y uvs *)
+    end
+  in Ext.intro_feq2 (sub_lam (sub_comp s1 s2)) (sub_comp (sub_lam s1) (sub_lam s2)) h
+
+and subst_comp_sub_comp (s1 s2 : sub) (c:comp)
+  : Lemma (requires True)
+    (ensures (subst_comp (sub_comp s1 s2) c == subst_comp s2 (subst_comp s1 c)))
+    (decreases %[1 ; is_renaming s1 ; is_renaming s2 ; 1 ; c])
+= match c with
+  | Tot_ t -> subst_sub_comp s1 s2 t
+  | Pure_ t wp -> subst_sub_comp s1 s2 t ; subst_sub_comp s1 s2 wp
+
+
+let o = sub_comp
+
+let sub_comp_assoc (s1 s2 s3:sub) : Lemma (s1 `o` (s2 `o` s3) == (s1 `o` s2) `o` s3)
+=
+  let sl = s1 `o` (s2 `o` s3) in
+  let sr = (s1 `o` s2) `o` s3 in
+  let h (y:var) (uvs:universes) : Lemma (sl y uvs == sr y uvs) =
+    subst_sub_comp s2 s3 (s1 y uvs)
+  in
+  Ext.intro_feq2 sl sr h
+
+(* Shifts *)
+
+let shift_up_above (x:var) (t:term) = subst (sub_inc_above x) t
+let shift_up = shift_up_above 0
+
+(* Environments *)
+
+type env = var -> Tot (option term)
+let empty : env = fun _ -> None
+
+let extend (g:env) (x:var) (t:term) : env =
+  fun (y:var) ->
+    if y < x then g y
+    else if y = x then Some (n, t)
+    else match g y with
+    | None -> None
+    | Some (n', t') -> Some (n', shift_up_above x t')
+
+(* Definitional equality *)
+
+type def_eq : term -> term -> Type0 =
+
+  (* Equivalence relation *)
+  | DEqRefl :
+    t:term ->
+    def_eq t t
+  | DEqSymm :
+    #t1:term ->
+    #t2:term ->
+    def_eq t1 t2 ->
+    def_eq t2 t1
+  | DEqTrans :
+    #t1:term ->
+    #t2:term ->
+    #t3:term ->
+    def_eq t1 t2 ->
+    def_eq t2 t3 ->
+    def_eq t1 t3
+
+  (* Congruences *)
+  | DEqApp :
+    #t1:term ->
+    #t1':term ->
+    #t2:term ->
+    #t2':term ->
+    def_eq t1 t2 ->
+    def_eq t1' t2' ->
+    def_eq (App t1 t2) (App t1' t2')
+  | DEqLam :
+    #t1:term ->
+    #t1':term ->
+    #t2:term ->
+    #t2':term ->
+    def_eq t1 t1' ->
+    def_eq t2 t2' ->
+    def_eq (Lam t1 t2) (Lam t1' t2')
+  | DEqProd :
+    #t:term ->
+    #t':term ->
+    #c:comp ->
+    #c':comp ->
+    def_eq t t' ->
+    def_eq_comp c c' ->
+    def_eq (Prod t c) (Prod t' c')
+  | DEqRefine :
+    #t:term ->
+    #t':term ->
+    #phi:term ->
+    #phi':term ->
+    def_eq t t' ->
+    def_eq phi phi' ->
+    def_eq (Refine t phi) (Refine t' phi')
+
+  (* Computation rules *)
+  | DEqBeta :
+    #t:term ->
+    #e1:term ->
+    #e2:term ->
+    def_eq (App (Lam t e1) e2) (subst_beta e2 e1)
+  | DEqNatElimZero :
+    #t:term ->
+    #e0:term ->
+    #esucc:term ->
+    def_eq (App (App (App (App (Const NatElim []) t) e0) esucc) (Const Zero [])) e0
+  | DEqNatElimSucc :
+    #t:term ->
+    #e0:term ->
+    #esucc:term ->
+    #n:term ->
+    def_eq (App (App (App (App (Const NatElim []) t) e0) esucc) (App (Const Succ []) n))
+           (App esucc (App (App (App (App (Const NatElim []) t) e0) esucc) n))
+  | DEqEqElimRefl :
+    #t:term ->
+    #erefl:term ->
+    def_eq (App (App (App (Const EqElim []) t) erefl) (Const Refl [])) erefl
+
+and def_eq_comp : comp -> comp -> Type0 =
+  | DEqCompTot :
+    #t:term ->
+    #t':term ->
+    def_eq t t' ->
+    def_eq_comp (Tot_ t) (Tot_ t')
+  | DEqCompPure :
+    #t:term ->
+    #t':term ->
+    #wp:term ->
+    #wp':term ->
+    def_eq t t' ->
+    def_eq wp wp' ->
+    def_eq_comp (Pure_ t wp) (Pure_ t wp')
+
+
+(* Typing *)
+
+(* type typing : env -> term -> term -> Type = *)
+(*  | TVar : *)
+(*   #g:env -> *)
+(*   valid g -> *)
+(*   x:var{Some? (g x)} -> *)
+(*   typing g (Var x []) *)
+(*  |  *)
